src/Bedrock/Field/Synthesis/Examples/BN446_PairingHelpers.v
@@ -1,0 +1,122 @@
+(** * BN446 Pairing Helper WP Proofs
+    Standalone WP correctness proofs for pairing helper functions
+    defined in BN446_Pairing.v:
+    - C1: bn446_Fp2_mul_fp (multiply Fp2 by Fp scalar)
+    - C3: bn446_load_gamma1_p2
+    - C4: bn446_load_gamma2_p2
+    - C5: bn446_load_w_frob_p2_c1
+    - C2: bn446_make_line
+*)
+
+From Stdlib Require Import Strings.String.
+From Stdlib Require Import ZArith.ZArith.
+Require Import bedrock2.NotationsCustomEntry.
+Require Import bedrock2.WeakestPrecondition.
+Require Import Rupicola.Lib.Api.
+Require Import coqutil.Word.Bitwidth64.
+Require Import bedrock2.BasicC64Semantics.
+Require Import Crypto.Arithmetic.PrimeFieldTheorems.
+Require Import Crypto.Bedrock.Specs.AbstractField.
+Require Import Crypto.Bedrock.Specs.PrimeField.
+Require Import Crypto.Bedrock.Field.Synthesis.New.WordByWordMontgomery.
+Require Import Crypto.Bedrock.Field.Synthesis.Examples.bn446_prime.
+Require Import Crypto.Bedrock.Field.Synthesis.Examples.bn446_prime_certif.
+Require Import Crypto.Bedrock.Field.Synthesis.Examples.bn446_felem_copy.
+Require Import Crypto.Bedrock.Field.FieldExtensions.QuadraticFieldExtensionsSpecs.
+Require Import Crypto.Bedrock.Field.FieldExtensions.QuadraticFieldExtensions.
+Require Import Crypto.Bedrock.Field.FieldExtensions.CubicFieldExtensionsSpecs.
+Require Import Crypto.Bedrock.Field.FieldExtensions.CubicFieldExtensions.
+Require Import Crypto.Bedrock.Field.FieldExtensions.DodecicFieldExtensionsSpecs.
+Require Import Crypto.Bedrock.Field.FieldExtensions.DodecicFieldExtensions.
+Require Import Crypto.Bedrock.Field.FieldExtensions.PairingFieldOps.
+Require Import Crypto.Bedrock.Field.FieldExtensions.WPTactics.
+Require Import Crypto.Bedrock.Field.Synthesis.Examples.BN446_Pairing.
+Require Import Crypto.Bedrock.Field.Synthesis.Examples.BLS12_CurveInstances.
+
+Import BinInt String List.ListNotations.
+
+Local Open Scope string_scope.
+Local Open Scope Z_scope.
+Local Open Scope list_scope.
+
+Section BN446_PairingHelpers.
+
+    Existing Instances
+      Defaults64.default_parameters
+      Defaults64.default_parameters_ok.
+
+    Let bn446_M_pos : positive := Eval vm_compute in (Z.to_pos bn446_prime.m).
+
+    Instance bn446_pf_params : PrimeFieldParameters := {|
+      PrimeField.M_pos := bn446_M_pos;
+      PrimeField.a24 := F.of_Z _ 0;
+      PrimeField.mul := "bn446_mul";
+      PrimeField.add := "bn446_add";
+      PrimeField.sub := "bn446_sub";
+      PrimeField.opp := "bn446_opp";
+      PrimeField.square := "bn446_square";
+      PrimeField.scmula24 := "bn446_scmula24";
+      PrimeField.inv := "bn446_inv";
+      PrimeField.from_bytes := "bn446_from_bytes";
+      PrimeField.to_bytes := "bn446_to_bytes";
+      PrimeField.select_znz := "bn446_select_znz";
+      PrimeField.felem_copy := "bn446_felem_copy";
+      PrimeField.from_word := "bn446_from_word";
+      PrimeField.from_list := "bn446_from_list";
+    |}.
+
+    Instance bn446_pf_params_ok : PrimeFieldParameters_ok.
+    Proof. constructor. exact prime_bn446. Qed.
+
+    Existing Instance prime_field_parameters.
+
+    Local Notation Fp := (F PrimeField.M_pos).
+    Local Notation Fp2 := ((Fp * Fp)%type).
+    Local Notation Fp6 := ((Fp2 * Fp2 * Fp2)%type).
+    Local Notation Fp12 := ((Fp6 * Fp6)%type).
+
+    Instance bn446_Fp_rep : AbstractField.FieldRepresentation (F:=Fp) :=
+      {| AbstractField.feval := @Field.feval _ _ _ _ _ bn446_frep;
+         AbstractField.feval_bytes := @Field.feval_bytes _ _ _ _ _ bn446_frep;
+         AbstractField.felem_size_in_words := @Field.felem_size_in_words _ _ _ _ _ bn446_frep;
+         AbstractField.encoded_felem_size_in_bytes := @Field.encoded_felem_size_in_bytes _ _ _ _ _ bn446_frep;
+         AbstractField.bytes_in_bounds := @Field.bytes_in_bounds _ _ _ _ _ bn446_frep;
+         AbstractField.bounds := @Field.bounds _ _ _ _ _ bn446_frep;
+         AbstractField.bounded_by := @Field.bounded_by _ _ _ _ _ bn446_frep;
+         AbstractField.loose_bounds := @Field.loose_bounds _ _ _ _ _ bn446_frep;
+         AbstractField.tight_bounds := @Field.tight_bounds _ _ _ _ _ bn446_frep |}.
+
+    Instance bn446_Fp_rep_ok : AbstractField.FieldRepresentation_ok (F:=Fp).
+    Proof.
+      constructor. intros X H.
+      cbv [bounded_by bn446_Fp_rep] in *.
+      cbv [Field.bounded_by bn446_frep field_representation
+           Signature.field_representation Representation.frep] in *.
+      exact H.
+    Defined.
+
+    Let bn446_beta : F PrimeField.M_pos := F.of_Z PrimeField.M_pos (-1).
+    Let bn446_xi_re : F PrimeField.M_pos := F.of_Z PrimeField.M_pos 2.
+    Let bn446_xi_im : F PrimeField.M_pos := F.of_Z PrimeField.M_pos 3.
+
+    Let fp2_prefix := "bn446_Fp2_".
+    Let fp6_prefix := "bn446_Fp6_".
+    Let fp12_prefix := "bn446_Fp12_".
+
+    Instance bn446_Fp2_params' : AbstractField.FieldParameters Fp2 :=
+      ltac:(let v := eval cbv [ext_Fp2_params append] in (ext_Fp2_params bn446_beta "bn446_") in exact v).
+    Instance bn446_Fp2_rep' : AbstractField.FieldRepresentation (F:=Fp2) :=
+      ltac:(let v := eval cbv [ext_Fp2_rep append] in (ext_Fp2_rep bn446_beta "bn446_") in exact v).
+    Instance bn446_Fp6_params' : AbstractField.FieldParameters Fp6 :=
+      ltac:(let v := eval cbv [ext_Fp6_params append] in (ext_Fp6_params bn446_beta bn446_xi_re bn446_xi_im "bn446_") in exact v).
+    Instance bn446_Fp6_rep' : AbstractField.FieldRepresentation (F:=Fp6) :=
+      ltac:(let v := eval cbv [ext_Fp6_rep append] in (ext_Fp6_rep bn446_beta bn446_xi_re bn446_xi_im "bn446_") in exact v).
+    Instance bn446_Fp12_params' : AbstractField.FieldParameters Fp12 :=
+      ltac:(let v := eval cbv [ext_Fp12_params append] in (ext_Fp12_params bn446_beta bn446_xi_re bn446_xi_im "bn446_") in exact v).
+    Instance bn446_Fp12_rep' : AbstractField.FieldRepresentation (F:=Fp12) :=
+      ltac:(let v := eval cbv [ext_Fp12_rep append] in (ext_Fp12_rep bn446_beta bn446_xi_re bn446_xi_im "bn446_") in exact v).
+
+    (* Placeholder: WP proofs for helper functions will follow the same pattern
+       as BN254_PairingHelpers.v, adapted for 7-limb Fp elements. *)
+
+End BN446_PairingHelpers.
