src/Spec/HashToCurveIsogenyProof.v
@@ -1,0 +1,325 @@
+(** * Isogeny correctness proof. *)
+
+From Stdlib Require Import ZArith BinPos List Bool Lia.
+Import ListNotations.
+Require Import Crypto.Spec.ModularArithmetic.
+Require Import Crypto.Arithmetic.ModularArithmeticTheorems.
+Require Import Crypto.Spec.HashToCurve.
+Require Import Crypto.Spec.HashToCurveFieldSetup.
+Require Import Crypto.Spec.HashToCurvePolyArith.
+Require Import Crypto.Spec.HashToCurveIsogenyCompute.
+Require Import Crypto.Spec.HashToCurveSWUProof.
+
+Local Open Scope Z_scope.
+Import HashToCurveIsogenyCompute.  (* Import p_Z as a shared Definition *)
+Local Notation fpoly cs x := (F.of_Z p_pos (poly_eval_Z cs x)).
+
+Lemma pe_cons2 : forall a b rest x,
+  poly_eval_Z (a :: b :: rest) x = a + x * poly_eval_Z (b :: rest) x.
+Proof. reflexivity. Qed.
+
+Lemma pe_cons_ne : forall c tail x,
+  tail <> [] -> poly_eval_Z (c :: tail) x = c + x * poly_eval_Z tail x.
+Proof. intros c [|t ts] x Hne; [contradiction|reflexivity]. Qed.
+
+Lemma poly_add_nonempty : forall p a f b g,
+  poly_add_Z p (a :: f) (b :: g) <> [].
+Proof. intros. simpl. destruct f, g; discriminate. Qed.
+
+Lemma poly_scale_nonempty : forall p c a f,
+  poly_scale_Z p c (a :: f) <> [].
+Proof. intros. unfold poly_scale_Z. simpl. discriminate. Qed.
+
+(* ================================================================== *)
+(** * Z-level polynomial evaluation correctness                        *)
+(* ================================================================== *)
+
+Lemma poly_add_Z_eval : forall f g x,
+  poly_eval_Z (poly_add_Z p_Z f g) x mod p_Z =
+  (poly_eval_Z f x + poly_eval_Z g x) mod p_Z.
+Proof.
+  induction f as [|a f' IH]; intros g x; [reflexivity|].
+  destruct g as [|b g'];
+    [change (poly_eval_Z [] x) with 0; rewrite Z.add_0_r; reflexivity|].
+  destruct f' as [|a2 f''], g' as [|b2 g''].
+  - simpl. rewrite Zmod_mod. reflexivity.
+  - simpl poly_add_Z. rewrite pe_cons2.
+    change (poly_eval_Z [a] x) with a. rewrite (pe_cons2 b b2 g'' x).
+    set (pe := poly_eval_Z (b2 :: g'') x).
+    rewrite Zplus_mod_idemp_l. f_equal. ring_simplify. reflexivity.
+  - simpl poly_add_Z. rewrite !pe_cons2.
+    change (poly_eval_Z [b] x) with b.
+    set (pe := poly_eval_Z (a2 :: f'') x).
+    rewrite Zplus_mod_idemp_l. f_equal. ring_simplify. reflexivity.
+  - change (poly_add_Z p_Z (a :: a2 :: f'') (b :: b2 :: g''))
+      with ((a + b) mod p_Z :: poly_add_Z p_Z (a2 :: f'') (b2 :: g'')).
+    rewrite (pe_cons_ne _ _ _ (poly_add_nonempty _ a2 f'' b2 g'')).
+    rewrite (pe_cons2 a a2 f'' x), (pe_cons2 b b2 g'' x).
+    (* LHS: ((a+b) mod p + x * pe_add) mod p *)
+    (* RHS: (a + x*pe_f + (b + x*pe_g)) mod p *)
+    (* Normalize LHS: idemp_l strips (a+b) mod p *)
+    rewrite Zplus_mod_idemp_l.
+    (* LHS: (a + b + x * pe_add) mod p *)
+    rewrite Zplus_mod, (Zmult_mod x).
+    rewrite IH.
+    rewrite <- (Zmult_mod x), <- Zplus_mod.
+    (* LHS: (a + b + x * (pe_f + pe_g)) mod p *)
+    f_equal.
+    set (pf := poly_eval_Z (a2 :: f'') x).
+    set (pg := poly_eval_Z (b2 :: g'') x).
+    clearbody pf pg. clear -pf pg a b x.
+    rewrite Z.mul_add_distr_l. ring_simplify. reflexivity.
+Qed.
+
+Lemma poly_scale_Z_eval : forall c f x,
+  poly_eval_Z (poly_scale_Z p_Z c f) x mod p_Z =
+  (c * poly_eval_Z f x) mod p_Z.
+Proof.
+  intros c f. induction f as [|a f' IH]; intro x.
+  - simpl. rewrite Z.mul_0_r. reflexivity.
+  - destruct f' as [|a2 f''].
+    + simpl. rewrite Zmod_mod. reflexivity.
+    + change (poly_scale_Z p_Z c (a :: a2 :: f''))
+        with ((c * a) mod p_Z :: poly_scale_Z p_Z c (a2 :: f'')).
+      rewrite (pe_cons_ne _ _ _ (poly_scale_nonempty _ c a2 f'')), (pe_cons2 a a2 f'' x).
+      set (pe_s := poly_eval_Z (poly_scale_Z p_Z c (a2 :: f'')) x).
+      set (pe := poly_eval_Z (a2 :: f'') x).
+      rewrite Zplus_mod, (Zmult_mod x pe_s). subst pe_s. rewrite IH.
+      rewrite <- (Zmult_mod x), <- Zplus_mod.
+      rewrite Zplus_mod_idemp_l. f_equal. subst pe. ring_simplify. reflexivity.
+Qed.
+
+Lemma poly_cons0_eval : forall f x,
+  poly_eval_Z (0 :: f) x mod p_Z = (x * poly_eval_Z f x) mod p_Z.
+Proof.
+  intros f x. destruct f as [|a f'].
+  - simpl. rewrite Z.mul_0_r. reflexivity.
+  - rewrite pe_cons2. rewrite Z.add_0_l. reflexivity.
+Qed.
+
+Lemma poly_mul_Z_eval : forall f g x,
+  poly_eval_Z (poly_mul_Z p_Z f g) x mod p_Z =
+  (poly_eval_Z f x * poly_eval_Z g x) mod p_Z.
+Proof.
+  induction f as [|a f' IH]; intros g x.
+  - reflexivity.
+  - change (poly_mul_Z p_Z (a :: f') g)
+      with (poly_add_Z p_Z (poly_scale_Z p_Z a g) (0 :: poly_mul_Z p_Z f' g)).
+    rewrite poly_add_Z_eval. rewrite Zplus_mod.
+    rewrite poly_scale_Z_eval, poly_cons0_eval.
+    set (pe_g := poly_eval_Z g x).
+    set (pe_mul := poly_eval_Z (poly_mul_Z p_Z f' g) x).
+    rewrite Zplus_mod, (Zmult_mod x pe_mul). subst pe_mul. rewrite IH.
+    set (pe_f := poly_eval_Z f' x).
+    rewrite <- (Zmult_mod x).
+    (* Reassemble: use Zplus_mod_idemp on both sides *)
+    rewrite !Zplus_mod_idemp_l, !Zplus_mod_idemp_r.
+    subst pe_f pe_g.
+    f_equal.
+    destruct f' as [|a2 f''].
+    + simpl poly_eval_Z. set (pg := poly_eval_Z g x).
+      clearbody pg. clear -pg a x. ring_simplify. reflexivity.
+    + rewrite pe_cons2. set (pe := poly_eval_Z (a2 :: f'') x).
+      set (pg := poly_eval_Z g x).
+      clearbody pe pg. clear -pe pg a x. ring_simplify. reflexivity.
+Qed.
+
+Lemma poly_pow_Z_eval : forall f n x,
+  poly_eval_Z (poly_pow_Z p_Z f n) x mod p_Z =
+  (Z.pow (poly_eval_Z f x) (Z.of_nat n)) mod p_Z.
+Proof.
+  intros f n. induction n as [|n' IH]; intro x.
+  - simpl. reflexivity.
+  - simpl poly_pow_Z. rewrite poly_mul_Z_eval.
+    set (pe := poly_eval_Z f x).
+    rewrite Zmult_mod. subst pe. rewrite IH.
+    set (pe := poly_eval_Z f x).
+    rewrite <- Zmult_mod.
+    rewrite Nat2Z.inj_succ, Z.pow_succ_r by lia. reflexivity.
+Qed.
+
+(* ================================================================== *)
+(** * F-level bridges via F.eq_to_Z_iff                                *)
+(* ================================================================== *)
+
+Lemma fpoly_add : forall f g x,
+  fpoly (poly_add_Z p_Z f g) x = @F.add p_pos (fpoly f x) (fpoly g x).
+Proof.
+  intros. apply F.eq_to_Z_iff.
+  rewrite F.to_Z_add, !F.to_Z_of_Z, Zplus_mod_idemp_l, Zplus_mod_idemp_r.
+  exact (poly_add_Z_eval f g x).
+Qed.
+
+Lemma fpoly_scale : forall c f x,
+  fpoly (poly_scale_Z p_Z c f) x = @F.mul p_pos (F.of_Z p_pos c) (fpoly f x).
+Proof.
+  intros. apply F.eq_to_Z_iff.
+  rewrite F.to_Z_mul, !F.to_Z_of_Z, Zmult_mod_idemp_l, Zmult_mod_idemp_r.
+  exact (poly_scale_Z_eval c f x).
+Qed.
+
+Lemma fpoly_mul : forall f g x,
+  fpoly (poly_mul_Z p_Z f g) x = @F.mul p_pos (fpoly f x) (fpoly g x).
+Proof.
+  intros. apply F.eq_to_Z_iff.
+  rewrite F.to_Z_mul, !F.to_Z_of_Z, Zmult_mod_idemp_l, Zmult_mod_idemp_r.
+  exact (poly_mul_Z_eval f g x).
+Qed.
+
+Lemma Zpow_mod_idemp : forall a p n, 0 <= n -> (a mod p) ^ n mod p = a ^ n mod p.
+Proof.
+  intros a p0 n Hn. rewrite <- (Z2Nat.id n Hn).
+  set (m := Z.to_nat n). clearbody m. clear.
+  induction m as [|m' IH]; [reflexivity|].
+  rewrite Nat2Z.inj_succ, !Z.pow_succ_r by lia.
+  rewrite Zmult_mod, IH, <- Zmult_mod, Zmult_mod_idemp_l. reflexivity.
+Qed.
+
+Lemma fpoly_pow : forall f n x,
+  fpoly (poly_pow_Z p_Z f n) x = F.pow (fpoly f x) (N.of_nat n).
+Proof.
+  intros. apply F.eq_to_Z_iff.
+  rewrite F.to_Z_pow, !F.to_Z_of_Z, nat_N_Z.
+  rewrite Zpow_mod_idemp by lia.
+  exact (poly_pow_Z_eval f n x).
+Qed.
+
+(* ================================================================== *)
+(** * Coefficient correspondences + isogeny identity                    *)
+(* ================================================================== *)
+
+Lemma iso_xnum_Z_eq : iso_xnum = map (F.of_Z p_pos) xnum_Z.
+Proof. reflexivity. Qed.
+Lemma iso_ynum_Z_eq : iso_ynum = map (F.of_Z p_pos) ynum_Z.
+Proof. reflexivity. Qed.
+Lemma iso_xden_monic_eq : iso_xden ++ [F.one] = map (F.of_Z p_pos) xden_Z.
+Proof. reflexivity. Qed.
+Lemma iso_yden_monic_eq : iso_yden ++ [F.one] = map (F.of_Z p_pos) yden_Z.
+Proof. reflexivity. Qed.
+
+Lemma curve_eprime_as_horner : forall x' : F p_pos,
+  cube x' +f iso_A *f x' +f iso_B =
+  horner_eval (map (F.of_Z p_pos) curve_eprime_Z) x'.
+Proof.
+  intro x'. unfold curve_eprime_Z. simpl map. simpl horner_eval.
+  change (F.of_Z p_pos iso_B_Z) with iso_B.
+  change (F.of_Z p_pos iso_A_Z) with iso_A.
+  Opaque iso_A iso_B. unfold cube, sqr. ring. Transparent iso_A iso_B.
+Qed.
+
+Lemma isogeny_identity_F : forall (x' : Fp),
+  ((cube x' +f iso_A *f x' +f iso_B) *f
+    sqr (horner_eval iso_ynum x') *f
+    cube (horner_eval_monic iso_xden x') =
+  cube (horner_eval iso_xnum x') *f
+    sqr (horner_eval_monic iso_yden x') +f
+  F.of_Z p_pos 4 *f
+    cube (horner_eval_monic iso_xden x') *f
+    sqr (horner_eval_monic iso_yden x'))%F.
+Proof.
+  intro x'.
+  rewrite curve_eprime_as_horner, iso_xnum_Z_eq, iso_ynum_Z_eq.
+  unfold horner_eval_monic.
+  rewrite iso_xden_monic_eq, iso_yden_monic_eq.
+  rewrite !horner_eval_of_Z.
+  assert (Hsqr : forall a : Fp, sqr a = F.pow a 2%N).
+  { intro a. unfold sqr. rewrite F.pow_2_r. reflexivity. }
+  assert (Hcube : forall a : Fp, cube a = F.pow a 3%N).
+  { intro a. unfold cube, sqr. rewrite F.pow_3_r. reflexivity. }
+  rewrite !Hsqr, !Hcube.
+  change 2%N with (N.of_nat 2). change 3%N with (N.of_nat 3).
+  rewrite <- (fpoly_pow ynum_Z 2), <- (fpoly_pow yden_Z 2).
+  rewrite <- (fpoly_pow xnum_Z 3), <- (fpoly_pow xden_Z 3).
+  (* Unify all Z.pos p_pos with IsogenyCompute.p_Z *)
+  change (Z.pos p_pos) with HashToCurveIsogenyCompute.p_Z.
+  rewrite <- ynum2_eq, <- yden2_eq, <- xnum3_eq, <- xden3_eq.
+  rewrite <- (fpoly_mul curve_eprime_Z ynum2_Z), <- curve_ynum2_eq.
+  rewrite <- (fpoly_mul curve_ynum2_Z xden3_Z), <- lhs_eq.
+  rewrite <- (fpoly_mul xnum3_Z yden2_Z), <- xnum3_yden2_eq.
+  rewrite <- (fpoly_scale 4 xden3_Z), <- scale4_xden3_eq.
+  rewrite <- (fpoly_mul scale4_xden3_Z yden2_Z), <- scale4_xden3_yden2_eq.
+  rewrite <- (fpoly_add xnum3_yden2_Z scale4_xden3_yden2_Z), <- rhs_eq.
+  apply poly_eval_mod_ext.
+  exact isogeny_poly_identity.
+Qed.
+
+(* ================================================================== *)
+(** * Isogeny correct for non-kernel points                            *)
+(* ================================================================== *)
+
+Theorem iso_map_correct : forall (x' y' : Fp),
+  on_curve_Eprime (x', y') ->
+  horner_eval_monic iso_xden x' <> 0f ->
+  horner_eval_monic iso_yden x' <> 0f ->
+  on_curve_E (iso_map (x', y')).
+Proof.
+  intros x' y' Hcurve Hxd Hyd.
+  unfold on_curve_Eprime in Hcurve.
+  unfold on_curve_E, iso_map, bls12_b.
+  set (xn := horner_eval iso_xnum x').
+  set (xd := horner_eval_monic iso_xden x').
+  set (yn := horner_eval iso_ynum x').
+  set (yd := horner_eval_monic iso_yden x').
+  assert (Hident := isogeny_identity_F x').
+  fold xn xd yn yd in Hident.
+  fold xd in Hxd. fold yd in Hyd.
+  rewrite <- Hcurve in Hident.
+  unfold sqr, cube in *.
+  clearbody xn xd yn yd.
+  clear Hcurve x'.
+  (* Goal: y'*yn*inv(yd) * (y'*yn*inv(yd)) = xn*inv(xd)*(xn*inv(xd))*(xn*inv(xd)) + of_Z 4 *)
+  (* Hident: y'*y'*(yn*yn)*(xd*xd*xd) = xn*xn*xn*(yd*yd) + of_Z 4*(xd*xd*xd)*(yd*yd) *)
+  (* Strategy: show Goal * (xd^3 * yd^2) = Hident, then cancel. *)
+  pose proof (Fp_mul_inv_r xd Hxd) as Hxdi.  (* xd * inv(xd) = 1 *)
+  pose proof (Fp_mul_inv_r yd Hyd) as Hydi.  (* yd * inv(yd) = 1 *)
+  pose proof (Fp_inv_nonzero xd Hxd) as Hixd. (* inv(xd) * xd = 1 *)
+  pose proof (Fp_inv_nonzero yd Hyd) as Hiyd. (* inv(yd) * yd = 1 *)
+  (* Cancel lemma *)
+  assert (Hcancel : forall a b c : Fp, c <> 0f -> a *f c = b *f c -> a = b).
+  { intros a0 b0 c0 Hc Hab.
+    assert (Hic := Fp_mul_inv_r c0 Hc).
+    assert (H0 : a0 *f c0 *f F.inv c0 = b0 *f c0 *f F.inv c0).
+    { f_equal. exact Hab. }
+    Opaque F.of_Z. (* prevent ring from normalizing big constants *)
+    replace (a0 *f c0 *f F.inv c0) with (a0 *f (c0 *f F.inv c0)) in H0 by ring.
+    replace (b0 *f c0 *f F.inv c0) with (b0 *f (c0 *f F.inv c0)) in H0 by ring.
+    rewrite Hic in H0.
+    replace (a0 *f 1f) with a0 in H0 by ring.
+    replace (b0 *f 1f) with b0 in H0 by ring.
+    Transparent F.of_Z. exact H0. }
+  set (C := xd *f xd *f xd *f (yd *f yd)).
+  assert (HC : C <> 0f).
+  { subst C. intro HC.
+    assert (Hmn := @mul_nonzero).
+    apply Hxd. destruct (F.eq_dec xd 0f); [assumption|exfalso].
+    apply Hyd. destruct (F.eq_dec yd 0f); [assumption|exfalso].
+    apply (Hmn (xd *f xd *f xd) (yd *f yd)).
+    - apply (Hmn (xd *f xd) xd); [apply (Hmn xd xd); assumption|assumption].
+    - apply (Hmn yd yd); assumption.
+    - exact HC. }
+  apply (Hcancel _ _ C HC).
+  (* Goal: LHS * C = RHS * C *)
+  (* LHS*C = y'*yn*inv(yd)*(y'*yn*inv(yd)) * xd^3*yd^2 *)
+  (*       = y'^2*yn^2 * (inv(yd)*yd)^2 * xd^3          [rearranging + simplifying] *)
+  (*       = y'^2*yn^2*xd^3                                [since inv(yd)*yd=1] *)
+  (* RHS*C = (xn*inv(xd)*(xn*inv(xd))*(xn*inv(xd))+4) * xd^3*yd^2 *)
+  (*       = xn^3*(inv(xd)*xd)^3*yd^2 + 4*xd^3*yd^2     [distributing + rearranging] *)
+  (*       = xn^3*yd^2 + 4*xd^3*yd^2                      [since inv(xd)*xd=1] *)
+  subst C.
+  Opaque F.of_Z.
+  (* Rewrite inv(xd)*xd = 1 and inv(yd)*yd = 1 *)
+  (* First, rearrange so that xd*inv(xd) and yd*inv(yd) are adjacent *)
+  (* Use 'enough' to provide Hident as a subtraction = 0, then field_simplify *)
+  Opaque F.of_Z.
+  field_simplify_eq; try assumption;
+    try (apply mul_nonzero; assumption);
+    try (apply mul_nonzero; [apply mul_nonzero|]; assumption).
+  field_simplify_eq in Hident; try assumption;
+    try (apply mul_nonzero; assumption);
+    try (apply mul_nonzero; [apply mul_nonzero|]; assumption).
+  etransitivity; [exact Hident|].
+  Transparent F.of_Z.
+  set (four := F.of_Z p_pos 4). clearbody four.
+  ring_simplify. reflexivity.
+  Unshelve. split; assumption.
+Qed.
